rt spec+proof: add sorted_ipc_queues invariant
This adds the invariant sorted_ipc_queues, which states that the ipc
queues are sorted by the priority of the TCB. More specifically,
the queues are nonincreasing with respect to the priority of the TCB.

This additionally uses the filter operation in the specification
of tcb_ep_append and tcb_ep_dequeue.

Signed-off-by: Michael McInerney <michael.mcinerney@proofcraft.systems>

spec/haskell/src/SEL4/Object/Endpoint.lhs
@@ -34,6 +34,7 @@ This module specifies the contents and behaviour of a synchronous IPC endpoint.
 
 > import Data.List
 > import Data.Maybe
+> import Data.Helpers (mapMaybe, distinct)
 
 \end{impdetails}
 
@@ -257,6 +258,7 @@ If a thread is blocking on an endpoint, then the endpoint is fetched and the thr
 >     ep <- getEndpoint epptr
 >     assert (not $ isIdle ep)
 >         "blockedCancelIPC: endpoint must not be idle"
+>     assert (distinct (epQueue ep)) "the endpoint queue of ep must be a list of distinct pointers"
 >     let queue' = delete tptr $ epQueue ep
 >     ep' <- return $ case queue' of
 >         [] -> IdleEP
@@ -309,6 +311,7 @@ If an endpoint is deleted, then every pending IPC operation using it must be can
 >             IdleEP ->
 >                 return ()
 >             _ -> do
+>                 assert (distinct (epQueue ep)) "the endpoint queue of ep must be a list of distinct pointers"
 >                 setEndpoint epptr IdleEP
 >                 forM_ (epQueue ep) (\t -> cancelAllIPC_loop_body t)
 >                 rescheduleRequired
@@ -327,6 +330,7 @@ If a badged endpoint is recycled, then cancel every pending send operation using
 >         IdleEP -> return ()
 >         RecvEP {} -> return ()
 >         SendEP queue -> do
+>             assert (distinct queue) "queue must be a list of distinct pointers"
 >             setEndpoint epptr IdleEP
 >             queue' <- (flip filterM queue) $ \t -> do
 >                 st <- getThreadState t
